coq/part-a.v
@@ -1,0 +1,1583 @@
+(* PoplMark Challenge, parts 1a and 2a
+   By Jerome Vouillon
+   March-May 2005
+
+   The proofs are written in Coq using de Bruijn indices.
+   The whole development took about twelve days.
+*)
+
+Set Implicit Arguments.
+Unset Strict Implicit.
+
+Require Import Arith.
+Require Import Omega.
+
+
+(*************************************************************************)
+(*                          Definition of Fsub                           *)
+(*************************************************************************)
+
+
+(*** Standard de Bruijn presentation of Fsub types and terms ***)
+
+Inductive typ : Set :=
+  | tvar : nat -> typ
+  | top : typ
+  | arrow : typ -> typ -> typ
+  | all : typ -> typ -> typ.
+
+Inductive term : Set :=
+  | var : nat -> term
+  | abs : typ -> term -> term
+  | app : term -> term -> term
+  | tabs : typ -> term -> term
+  | tapp : term -> typ -> term.
+
+(****)
+
+(*** Shiftings and substitutions ***)
+
+Fixpoint tshift (X : nat) (T : typ) {struct T} : typ :=
+  match T with
+  | tvar Y      => tvar (if le_gt_dec X Y then 1 + Y else Y)
+  | top         => top
+  | arrow T1 T2 => arrow (tshift X T1) (tshift X T2)
+  | all T1 T2   => all (tshift X T1) (tshift (1 + X) T2)
+  end.
+
+Fixpoint shift (x : nat) (t : term) {struct t} : term :=
+  match t with
+  | var y      => var (if le_gt_dec x y then 1 + y else y)
+  | abs T1 t2  => abs T1 (shift (1 + x) t2)
+  | app t1 t2  => app (shift x t1) (shift x t2)
+  | tabs T1 t2 => tabs T1 (shift x t2)
+  | tapp t1 T2 => tapp (shift x t1) T2
+  end.
+
+Fixpoint shift_typ (X : nat) (t : term) {struct t} : term :=
+  match t with
+  | var y      => var y
+  | abs T1 t2  => abs (tshift X T1) (shift_typ X t2)
+  | app t1 t2  => app (shift_typ X t1) (shift_typ X t2)
+  | tabs T1 t2 => tabs (tshift X T1) (shift_typ (1 + X) t2)
+  | tapp t1 T2 => tapp (shift_typ X t1) (tshift X T2)
+  end.
+
+Fixpoint tsubst (T : typ) (X : nat) (T' : typ) {struct T} : typ :=
+  match T with
+  | tvar Y =>
+      match lt_eq_lt_dec Y X with
+      | inleft (left _)  => tvar Y
+      | inleft (right _) => T'
+      | inright _        => tvar (Y - 1)
+      end
+  | top         => top
+  | arrow T1 T2 => arrow (tsubst T1 X T') (tsubst T2 X T')
+  | all T1 T2   => all (tsubst T1 X T') (tsubst T2 (1 + X) (tshift 0 T'))
+  end.
+
+Fixpoint subst (t : term) (x : nat) (t' : term) {struct t} : term :=
+  match t with
+  | var y =>
+      match lt_eq_lt_dec y x with
+      | inleft (left _)  => var y
+      | inleft (right _) => t'
+      | inright _        => var (y - 1)
+      end
+  | abs T1 t2  => abs T1 (subst t2 (1 + x) (shift 0 t'))
+  | app t1 t2  => app (subst t1 x t') (subst t2 x t')
+  | tabs T1 t2 => tabs T1 (subst t2 x (shift_typ 0 t'))
+  | tapp t1 T2 => tapp (subst t1 x t') T2
+  end.
+
+Fixpoint subst_typ (t : term) (X : nat) (T : typ) {struct t} : term :=
+  match t with
+  | var y      => var y
+  | abs T1 t2  => abs (tsubst T1 X T) (subst_typ t2 X T)
+  | app e1 e2  => app (subst_typ e1 X T) (subst_typ e2 X T)
+  | tabs T1 e1 => tabs (tsubst T1 X T) (subst_typ e1 (1 + X) (tshift 0 T))
+  | tapp e1 T2 => tapp (subst_typ e1 X T) (tsubst T2 X T)
+  end.
+
+(****)
+
+(*** Contexts ***)
+
+(* We define the contexts [env] and the two functions [get_bound] and
+   [get_var] which access the context. *)
+
+Inductive env : Set :=
+  | empty : env
+  | evar : env -> typ -> env
+  | ebound : env -> typ -> env.
+
+Definition opt_map (A B : Set) (f : A -> B) (x : option A) :=
+  match x with
+  | Some x => Some (f x)
+  | None => None
+  end.
+
+Fixpoint get_bound (e : env) (X : nat) {struct e} : option typ :=
+  match e with
+    empty     => None
+  | evar e' _ => get_bound e' X
+  | ebound e' T =>
+      opt_map (tshift 0)
+        (match X with
+         | O    => Some T
+         | S X' => get_bound e' X'
+         end)
+  end.
+
+Fixpoint get_var (e : env) (x : nat) {struct e} : option typ :=
+  match e with
+    empty       => None
+  | ebound e' _ => opt_map (tshift 0) (get_var e' x)
+  | evar e' T =>
+      match x with
+      | O    => Some T
+      | S x' => get_var e' x'
+      end
+  end.
+
+(****)
+
+(*** Well-formedness conditions ***)
+
+(* The variables must all be bound *)
+
+Fixpoint wf_typ (e : env) (T : typ) {struct T} : Prop :=
+  match T with
+  | tvar X      => get_bound e X <> None
+  | top         => True
+  | arrow T1 T2 => wf_typ e T1 /\ wf_typ e T2
+  | all T1 T2   => wf_typ e T1 /\ wf_typ (ebound e T1) T2
+  end.
+
+Fixpoint wf_term (e : env) (t : term) {struct t} : Prop :=
+  match t with
+  | var x      => get_var e x <> None
+  | abs T1 t2  => wf_typ e T1  /\ wf_term (evar e T1) t2
+  | app t1 t2  => wf_term e t1 /\ wf_term e t2
+  | tabs T1 t2 => wf_typ e T1  /\ wf_term (ebound e T1) t2
+  | tapp t1 T2 => wf_term e t1 /\ wf_typ e T2
+  end.
+
+Fixpoint wf_env (e : env) : Prop :=
+  match e with
+    empty      => True
+  | evar e T   => wf_typ e T /\ wf_env e
+  | ebound e T => wf_typ e T /\ wf_env e
+  end.
+
+(****)
+
+(*** Subtyping relation ***)
+
+(* In the definition of the subtyping and typing relations, we insert
+   some well-formedness condition that ensure that all environments,
+   types and terms occuring in these relations are well-formed. The
+   lemmas [sub_wf] and [typing_wf] show that this is indeed the case.
+
+   We inserted as few well-formedness condition as possible in order
+   to reduce the number of time we need to prove that a
+   well-formedness condition holds when building a derivation.
+*)
+
+Inductive sub : env -> typ -> typ -> Prop :=
+  | SA_Top :
+      forall (e : env) (S : typ), wf_env e -> wf_typ e S -> sub e S top
+  | SA_Refl_TVar :
+      forall (e : env) (X : nat),
+      wf_env e -> wf_typ e (tvar X) -> sub e (tvar X) (tvar X)
+  | SA_Trans_TVar :
+      forall (e : env) (X : nat) (T U : typ),
+      get_bound e X = Some U -> sub e U T -> sub e (tvar X) T
+  | SA_Arrow :
+      forall (e : env) (T1 T2 S1 S2 : typ),
+      sub e T1 S1 -> sub e S2 T2 -> sub e (arrow S1 S2) (arrow T1 T2)
+  | SA_All :
+      forall (e : env) (T1 T2 S1 S2 : typ),
+      sub e T1 S1 -> sub (ebound e T1) S2 T2 -> sub e (all S1 S2) (all T1 T2).
+
+(****)
+
+(*** Typing relation ***)
+
+Inductive typing : env -> term -> typ -> Prop :=
+  | T_Var :
+      forall (e : env) (x : nat) (T : typ),
+      wf_env e -> get_var e x = Some T -> typing e (var x) T
+  | T_Abs :
+      forall (e : env) (t : term) (T1 T2 : typ),
+      typing (evar e T1) t T2 ->
+      typing e (abs T1 t) (arrow T1 T2)
+  | T_App :
+      forall (e : env) (t1 t2 : term) (T11 T12 : typ),
+      typing e t1 (arrow T11 T12) ->
+      typing e t2 T11 -> typing e (app t1 t2) T12
+  | T_Tabs :
+      forall (e : env) (t : term) (T1 T2 : typ),
+      typing (ebound e T1) t T2 -> typing e (tabs T1 t) (all T1 T2)
+  | T_Tapp :
+      forall (e : env) (t1 : term) (T11 T12 T2 : typ),
+      typing e t1 (all T11 T12) ->
+      sub e T2 T11 -> typing e (tapp t1 T2) (tsubst T12 0 T2)
+  | T_Sub :
+      forall (e : env) (t : term) (T1 T2 : typ),
+      typing e t T1 -> sub e T1 T2 -> typing e t T2.
+
+(****)
+
+(*** Reduction rules ***)
+
+Definition value (t : term) :=
+  match t with
+  | abs _ _  => True
+  | tabs _ _ => True
+  | _        => False
+  end.
+
+Inductive ctx : Set :=
+    c_hole : ctx
+  | c_appfun : ctx -> term -> ctx
+  | c_apparg : forall (t : term), value t -> ctx -> ctx
+  | c_typefun : ctx -> typ -> ctx.
+
+Fixpoint ctx_app (c : ctx) (t : term) {struct c} : term :=
+  match c with
+    c_hole           => t
+  | c_appfun c' t'   => app (ctx_app c' t) t'
+  | c_apparg t' _ c' => app t' (ctx_app c' t)
+  | c_typefun c' T   => tapp (ctx_app c' t) T
+  end.
+
+Inductive red : term -> term -> Prop :=
+  | E_AppAbs :
+      forall (t11 : typ) (t12 t2 : term),
+      value t2 -> red (app (abs t11 t12) t2) (subst t12 0 t2)
+  | E_TappTabs :
+      forall (t11 t2 : typ) (t12 : term),
+      red (tapp (tabs t11 t12) t2) (subst_typ t12 0 t2)
+  | E_Ctx :
+      forall (c : ctx) (t1 t1' : term),
+      red t1 t1' -> red (ctx_app c t1) (ctx_app c t1').
+
+
+(*************************************************************************)
+(*                            General lemmas                             *)
+(*************************************************************************)
+
+
+(*** Commutation properties of shifting and substitution ***)
+
+Ltac tvar_case :=
+  unfold tshift; unfold tsubst; fold tshift; fold tsubst;
+  match goal with
+  | |- ?x =>
+      match x with
+      | context [le_gt_dec ?n ?n'] =>
+          case (le_gt_dec n n')
+      | context C [(lt_eq_lt_dec ?n ?n')] =>
+          case (lt_eq_lt_dec n n'); [intro s; case s; clear s | idtac ]
+      end
+  end.
+
+Ltac common_cases n T :=
+  simpl; generalize n; clear n; induction T; intros n''; intros;
+    [ repeat tvar_case;
+      simpl; trivial; try (intros; apply f_equal with (f := tvar); omega);
+      try (intros; assert False; [ omega | contradiction ])
+    | trivial
+    | simpl; apply f_equal2 with (f := arrow); trivial
+    | simpl; apply f_equal2 with (f := all); trivial ].
+
+Lemma tsubst_tshift_prop :
+  forall (n : nat) (T T' : typ), T = tsubst (tshift n T) n T'.
+intros n T; common_cases n T.
+Qed.
+
+Lemma tshift_tshift_prop_1 :
+  forall (n n' : nat) (T : typ),
+  tshift n (tshift (n + n') T) = tshift (1 + (n + n')) (tshift n T).
+intros n n' T; common_cases n T; exact (IHT2 (S n'')).
+Qed.
+
+Lemma tshift_tsubst_prop_1 :
+  forall (n n' : nat) (T T' : typ),
+  tshift n (tsubst T (n + n') T') =
+  tsubst (tshift n T) (1 + n + n') (tshift n T').
+intros n n' T; common_cases n T;
+rewrite (tshift_tshift_prop_1 0 n''); apply (IHT2 (S n'')).
+Qed.
+
+Lemma tshift_tsubst_prop_2 :
+  forall (n n' : nat) (T T' : typ),
+  (tshift (n + n') (tsubst T n T')) =
+  (tsubst (tshift (1 + n + n') T) n (tshift (n + n') T')).
+intros n n' T; common_cases n T;
+rewrite (tshift_tshift_prop_1 0 (n'' + n')); apply (IHT2 (S n'')).
+Qed.
+
+Lemma tsubst_tsubst_prop :
+  forall (n n' : nat) (T U V : typ),
+  (tsubst (tsubst T n U) (n + n') V) =
+  (tsubst (tsubst T (1 + n + n') (tshift n V)) n (tsubst U (n + n') V)).
+intros n n' T; common_cases n T;
+  [ intros; apply tsubst_tshift_prop
+  | rewrite (tshift_tsubst_prop_1 0 (n'' + n'));
+    rewrite (tshift_tshift_prop_1 0 n'');
+    apply (IHT2 (S n'')) ].
+Qed.
+
+(****)
+
+(*** Some properties of the well-formedness conditions *)
+
+Lemma wf_typ_env_weaken :
+  forall (T : typ) (e e' : env),
+  (forall (X : nat), get_bound e' X = None -> get_bound e X = None) ->
+  wf_typ e T -> wf_typ e' T.
+induction T; simpl; auto; intros e e' H (H1, H2); split;
+  [ apply (IHT1 _ _ H H1)
+  | apply (IHT2 _ _ H H2)
+  | apply (IHT1 _ _ H H1)
+  | apply IHT2 with (2 := H2); induction X;
+      [ trivial
+      | simpl; intro H3; rewrite H; trivial;
+        generalize H3; case (get_bound e' X); simpl; trivial;
+        intros; discriminate ] ].
+Qed.
+
+Lemma wf_typ_extensionality :
+  forall (T : typ) (e e' : env),
+  (forall (X : nat), get_bound e X = get_bound e' X) ->
+  wf_typ e T -> wf_typ e' T.
+intros T e e' H1 H2; apply wf_typ_env_weaken with (2 := H2);
+intros n H3; rewrite H1; trivial.
+Qed.
+
+(****)
+
+(*** Removal of a term variable binding ***)
+
+(*
+   This corresponds to the environment operation
+      E, x : T, E'  |-->  E.
+*)
+
+Fixpoint remove_var (e : env) (x : nat) {struct e} : env :=
+  match e with
+  | empty       => empty
+  | ebound e' T => ebound (remove_var e' x) T
+  | evar e' T =>
+      match x with
+      | O   => e'
+      | S x => evar (remove_var e' x) T
+      end
+  end.
+
+Lemma get_var_remove_var_lt :
+  forall (e : env) (x x' : nat),
+  x < x' -> get_var (remove_var e x') x = get_var e x.
+induction e; simpl; trivial; intros n n' H;
+  [ induction n';
+      [ inversion H
+      | clear IHn'; induction n; simpl; trivial;
+        apply IHe; omega ]
+  | apply f_equal with (f := opt_map (tshift 0)); auto ].
+Qed.
+
+Lemma get_var_remove_var_ge :
+  forall (e : env) (x x' : nat),
+  x >= x' -> get_var (remove_var e x') x = get_var e (1 + x).
+induction e; simpl; trivial; intros n n' H;
+  [ induction n'; trivial;
+    clear IHn'; induction n;
+      [ inversion H
+      | simpl; apply (IHe n); omega ]
+  | apply f_equal with (f := opt_map (tshift 0)); apply (IHe n); trivial ].
+Qed.
+
+Lemma get_bound_remove_var :
+  forall (e : env) (X x': nat), get_bound e X = get_bound (remove_var e x') X.
+induction e; simpl; trivial; intros n n';
+  [ induction n'; simpl; trivial
+  | induction n; trivial;
+    apply f_equal with (f := opt_map (tshift 0)); trivial ].
+Qed.
+
+Lemma wf_typ_remove_var :
+  forall (e : env) (x : nat) (T : typ),
+  wf_typ e T -> wf_typ (remove_var e x) T.
+intros e n T; apply wf_typ_extensionality;
+intro n'; apply get_bound_remove_var.
+Qed.
+
+Lemma wf_typ_insert_var :
+  forall (e : env) (n : nat) (T : typ),
+  wf_typ (remove_var e n) T -> wf_typ e T.
+intros e n T; apply wf_typ_extensionality; intro n';
+apply sym_eq; apply get_bound_remove_var.
+Qed.
+
+Lemma wf_env_remove_var :
+  forall (e : env) (x : nat), wf_env e -> wf_env (remove_var e x).
+induction e; simpl; trivial;
+  [ intros n (H1, H2); induction n; trivial;
+    simpl; split; auto; apply wf_typ_remove_var; trivial
+  | intros n (H1, H2); split; auto; apply wf_typ_remove_var; trivial ].
+Qed.
+
+(****)
+
+(*** Insertion of a type variable binding in an environment ****)
+
+(*
+   This corresponds to the environment operation
+       E, E'  |-->  E, X <: T, E'.
+   Note that all type variable in E' has to be shifted.
+*)
+
+Inductive insert_bound : nat -> env -> env -> Prop :=
+    ib_here :
+      forall (T : typ) (e : env), wf_typ e T -> insert_bound 0 e (ebound e T)
+  | ib_var :
+      forall (X : nat) (T : typ) (e e' : env),
+      insert_bound X e e' ->
+      insert_bound X (evar e T) (evar e' (tshift X T))
+  | ib_bound :
+      forall (X : nat) (T : typ) (e e' : env),
+      insert_bound X e e' ->
+      insert_bound (1 + X) (ebound e T) (ebound e' (tshift X T)).
+
+Lemma get_bound_insert_bound_ge :
+  forall (X X' : nat) (e e' : env),
+  insert_bound X' e e' -> X' <= X ->
+  get_bound e' (1 + X) = opt_map (tshift X') (get_bound e X).
+simpl; intros n n' e e' H; generalize n; clear n; induction H; simpl; trivial;
+intros n' H1; induction n'; simpl;
+  [ inversion H1
+  | clear IHn'; rewrite IHinsert_bound; try omega;
+    case (get_bound e n'); simpl; trivial;
+    intro T''; apply f_equal with (f := @Some typ);
+    apply (tshift_tshift_prop_1 0 X) ].
+Qed.
+
+Lemma get_bound_insert_bound_lt :
+  forall (X X' : nat) (e e' : env),
+  insert_bound X' e e' -> X < X' ->
+  get_bound e' X = opt_map (tshift X') (get_bound e X).
+intros n n' e e' H; generalize n; clear n; induction H; simpl; trivial;
+  [ intros n H1; inversion H1
+  | intros n' H1; induction n';
+      [ simpl; apply f_equal with (f := @Some typ);
+        apply (tshift_tshift_prop_1 0 X)
+      | clear IHn'; rewrite IHinsert_bound; try omega;
+        case (get_bound e n'); simpl; trivial;
+        intro T''; apply f_equal with (f := @Some typ);
+        apply (tshift_tshift_prop_1 0 X) ] ].
+Qed.
+
+Lemma get_var_insert_bound :
+  forall (x X' : nat) (e e' : env),
+  insert_bound X' e e' -> get_var e' x = opt_map (tshift X') (get_var e x).
+intros n n' e e' H; generalize n; clear n; induction H; simpl; intro n';
+  [ trivial
+  | induction n'; trivial
+  | rewrite IHinsert_bound; case (get_var e n'); simpl; trivial;
+    intro T'; apply f_equal with (f := @Some typ);
+    apply (tshift_tshift_prop_1 0 X) ].
+Qed.
+
+Lemma insert_bound_wf_typ :
+  forall (T : typ) (X : nat) (e e' : env),
+  insert_bound X e e' -> wf_typ e T -> wf_typ e' (tshift X T).
+induction T;
+  [ unfold tshift; fold tshift; intros n' e e' H1 H2; case (le_gt_dec n' n);
+      [ intro H3; unfold wf_typ; rewrite (get_bound_insert_bound_ge H1 H3);
+        intro H4; apply H2; induction (get_bound e n); trivial; discriminate
+      | intro H3; simpl; rewrite (get_bound_insert_bound_lt H1 H3);
+        intro H4; apply H2; induction (get_bound e n); trivial; discriminate ]
+  | trivial
+  | simpl; intros n e e' H1 (H2, H3); eauto
+  | simpl; intros n e e' H1 (H2, H3); split;
+      [ apply (IHT1 _ _ _ H1 H2)
+      | apply IHT2 with (e := (ebound e T1)); trivial;
+        exact (ib_bound T1 H1) ] ].
+Qed.
+
+Lemma insert_bound_wf_env :
+  forall (X : nat) (e e' : env),
+  insert_bound X e e' -> wf_env e -> wf_env e'.
+intros n e e' H; induction H; simpl; auto;
+intros (H1, H2); split; auto; exact (insert_bound_wf_typ H H1).
+Qed.
+
+(****)
+
+(*** More properties of the well-formedness conditions *)
+
+Lemma wf_typ_weakening_bound :
+  forall (e : env) (T U : typ),
+  wf_typ e T -> wf_typ e U -> wf_typ (ebound e U) (tshift 0 T).
+intros e T U H1 H2; apply insert_bound_wf_typ with (2 := H1);
+apply ib_here; trivial.
+Qed.
+
+Lemma wf_typ_weakening_var :
+  forall (e : env) (T U : typ),
+  wf_typ e U -> wf_typ (evar e T) U.
+intros e T U H; apply wf_typ_env_weaken with (2 := H); simpl; trivial.
+Qed.
+
+Lemma wf_typ_strengthening_var :
+  forall (e : env) (T U : typ),
+  wf_typ (evar e T) U -> wf_typ e U.
+intros e T U H; apply wf_typ_env_weaken with (2 := H); simpl; trivial.
+Qed.
+
+Lemma wf_typ_ebound :
+  forall (T U V : typ) (e : env),
+  wf_typ (ebound e U) T -> wf_typ (ebound e V) T.
+intros T U V e; apply wf_typ_env_weaken; intro X; induction X;
+  [ intros; discriminate
+  | trivial ].
+Qed.
+
+Lemma get_var_wf :
+  forall (e : env) (n : nat) (T : typ),
+  wf_env e -> get_var e n = Some T -> wf_typ e T.
+induction e; simpl;
+  [ intros; discriminate
+  | induction n; intros T (H1, H2) E;
+      [ injection E; clear E; intro E;
+        rewrite <- E; exact (wf_typ_weakening_var t H1)
+      | apply wf_typ_weakening_var; eauto ]
+  | intros n T (H1, H2) E; assert (H3 := IHe n); clear IHe;
+    induction (get_var e n);
+      [ simpl in E; injection E; clear E; intro E; rewrite <- E;
+        apply wf_typ_weakening_bound with (2 := H1); apply H3 with (1 := H2);
+        trivial
+      | discriminate ] ].
+Qed.
+
+
+(*************************************************************************)
+(*                       Transitivity of subtyping                       *)
+(*************************************************************************)
+
+
+(*** Subtyping relation well-formedness ***)
+
+Lemma sub_wf :
+  forall (e : env) (T U : typ),
+  sub e T U -> wf_env e /\ wf_typ e T /\ wf_typ e U.
+intros e T U H; induction H; repeat split; simpl; trivial; try tauto;
+  [ rewrite H; discriminate
+  | apply wf_typ_ebound with (U := T1); tauto ].
+Qed.
+
+(****)
+
+(*** A.1 Lemma [Reflexivity] ***)
+
+Lemma sub_reflexivity :
+  forall (e : env) (T : typ), wf_env e -> wf_typ e T -> sub e T T.
+intros e T; generalize e; clear e; induction T; intros e H1 H2;
+  [ apply SA_Refl_TVar; trivial
+  | apply SA_Top; trivial
+  | apply SA_Arrow;
+      [ exact (IHT1 _ H1 (proj1 H2))
+      | exact (IHT2 _ H1 (proj2 H2)) ]
+  | apply SA_All;
+      [ exact (IHT1 _ H1 (proj1 H2))
+      | apply IHT2 with (2 := (proj2 H2)); simpl; simpl in H2; tauto ] ].
+Qed.
+
+(****)
+
+(*** A.2 Lemma [Permutation and Weakening] ***)
+(*** A.5 Lemma [Weakening for Subtyping and Typing] (subtyping part) ***)
+
+(*
+   Our proof does not make use of any permutation lemma.
+   We only use one-step weakening with a variable inserted anywhere in
+   the environment.
+   The shifting is needed as a type variable binding is inserted in
+   the environment.
+*)
+
+Lemma sub_weakening_bound_ind :
+  forall (e e' : env) (X : nat) (U V : typ),
+  insert_bound X e e' -> sub e U V -> sub e' (tshift X U) (tshift X V).
+intros e e' X U V H1 H2; generalize X e' H1; clear X e' H1;
+induction H2; intros X' e' H1; simpl;
+  [ apply SA_Top;
+      [ exact (insert_bound_wf_env H1 H)
+      | exact (insert_bound_wf_typ H1 H0) ]
+  | apply SA_Refl_TVar;
+      [ exact (insert_bound_wf_env H1 H)
+      | exact (insert_bound_wf_typ H1 H0) ]
+  | apply SA_Trans_TVar with (2 := (IHsub X' e' H1));
+    case (le_gt_dec X' X); intro H3;
+      [ change (S X) with (1 + X); trivial;
+        rewrite get_bound_insert_bound_ge with (1 := H1) (2 := H3);
+        rewrite H; trivial
+      | rewrite get_bound_insert_bound_lt with (1 := H1) (2 := H3);
+        rewrite H; trivial ]
+  | apply SA_Arrow; auto
+  | apply SA_All; auto;
+    exact (IHsub2 (1 + X') _ (ib_bound T1 H1)) ].
+Qed.
+
+Lemma sub_weakening_bound :
+  forall (e : env) (T U V : typ),
+  wf_typ e V -> sub e T U -> sub (ebound e V) (tshift 0 T) (tshift 0 U).
+intros e T U V H0 H; apply sub_weakening_bound_ind with (2 := H);
+apply ib_here; trivial.
+Qed.
+
+(*
+   Rather than proving the weakening property for term variable
+   bindings by induction on a derivation on a derivation (as in the
+   paper proof), we prove the more general result that the subtyping
+   relation does not depend on the term variable bindings.  Then, this
+   intermediate result can be used for proving strengthening.
+*)
+
+Lemma sub_extensionality :
+  forall (e e' : env) (U V : typ),
+  (forall (X : nat), (get_bound e X) = (get_bound e' X)) -> wf_env e' ->
+  sub e U V -> sub e' U V.
+intros e e' U V H0 H1 H2; generalize e' H0 H1; clear e' H0 H1;
+induction H2; intros e' H3 H1;
+  [ apply SA_Top; trivial; exact (wf_typ_extensionality H3 H0)
+  | apply SA_Refl_TVar; trivial; exact (wf_typ_extensionality H3 H0)
+  | rewrite H3 in H; apply SA_Trans_TVar with (1 := H); auto
+  | apply SA_Arrow; auto
+  | apply SA_All; auto;
+    apply IHsub2 with (e' := (ebound e' T1));
+      [ intro X; induction X; simpl; trivial; rewrite H3; trivial
+      | simpl; split; trivial;
+        apply wf_typ_extensionality with (1 := H3);
+        exact (proj1 (proj2 (sub_wf H2_))) ] ].
+Qed.
+
+Lemma sub_weakening_var_ind :
+  forall (e : env) (x : nat) (U V : typ),
+  wf_env e -> sub (remove_var e x) U V -> sub e U V.
+intros e x U V H1; apply sub_extensionality; trivial;
+intro X; apply sym_eq; apply get_bound_remove_var.
+Qed.
+
+Lemma sub_weakening_var :
+  forall (e : env) (T U V : typ),
+  wf_typ e V -> sub e T U -> sub (evar e V) T U.
+intros e T U V H1 H2; generalize H2; apply sub_extensionality; trivial;
+simpl; split; trivial; exact (proj1 (sub_wf H2)).
+Qed.
+
+(****)
+
+(*** Relation "E' is a narrow of E" ***)
+
+(*
+   The environments E,X <: Q,E' and E,X<:P,E' are in a narrowing relation
+   if E |- P <: Q.
+*)
+
+Inductive narrow : nat -> env -> env -> Prop :=
+    narrow_0 :
+      forall (e : env) (T T' : typ),
+      sub e T' T -> narrow 0 (ebound e T) (ebound e T')
+  | narrow_extend_bound :
+      forall (e e' : env) (T : typ) (X : nat),
+      wf_typ e' T -> narrow X e e' ->
+      narrow (1 + X) (ebound e T) (ebound e' T)
+  | narrow_extend_var :
+      forall (e e' : env) (T : typ) (X : nat),
+      wf_typ e' T -> narrow X e e' -> narrow X (evar e T) (evar e' T).
+
+Lemma get_bound_narrow_ne :
+  forall (X X' : nat) (e e' : env),
+  narrow X e e' -> X' <> X -> get_bound e X' = get_bound e' X'.
+intros n n' e e' H; generalize n'; clear n'; induction H; intros n' H1; simpl;
+  [ induction n'; trivial; case H1; trivial
+  | induction n'; trivial; rewrite IHnarrow; trivial; omega
+  | auto ].
+Qed.
+
+Lemma get_bound_narrow_eq :
+  forall (X : nat) (e e' : env),
+  narrow X e e' ->
+  exists T, exists T',
+  get_bound e X = Some T /\ get_bound e' X = Some T' /\ sub e' T' T.
+intros n e e' H; induction H;
+  [ exists (tshift 0 T); exists (tshift 0 T'); repeat split;
+    apply sub_weakening_bound; trivial; exact (proj1 (proj2 (sub_wf H)))
+  | generalize IHnarrow; intros (Q, (P, (H1, (H2, H3))));
+    exists (tshift 0 Q); exists (tshift 0 P); simpl; repeat split;
+      [ rewrite H1; trivial
+      | rewrite H2; trivial
+      | apply sub_weakening_bound; trivial ]
+  | generalize IHnarrow; intros (Q, (P, (H1, (H2, H3))));
+    exists Q; exists P; repeat split; trivial;
+    apply sub_weakening_var; trivial ].
+Qed.
+
+Lemma get_var_narrow :
+  forall (X x' : nat) (e e' : env),
+  narrow X e e' -> get_var e x' = get_var e' x'.
+intros n n' e e' H; generalize n'; clear n'; induction H;
+  [ trivial
+  | simpl; intros n'; rewrite IHnarrow; trivial
+  | simpl; induction n'; trivial ].
+Qed.
+
+Lemma narrow_wf_typ :
+  forall (e e' : env) (T : typ) (X : nat),
+  narrow X e e' -> wf_typ e T -> wf_typ e' T.
+intros e e' T n H1 H2;
+apply wf_typ_env_weaken with (2 := H2); intros n' H3;
+case (eq_nat_dec n' n);
+  [ intros E; rewrite E in H3;
+    generalize (get_bound_narrow_eq H1);
+    intros (Q, (P, (H4, (H5, H6)))); rewrite H5 in H3; discriminate
+  | intro H4; rewrite (get_bound_narrow_ne H1 H4); trivial ].
+Qed.
+
+Lemma narrow_wf_env :
+  forall (e e' : env) (X : nat),
+  narrow X e e' -> wf_env e -> wf_env e'.
+intros e e' n H; induction H; simpl;
+intros (H1, H2); split; auto;
+exact (proj1 (proj2 (sub_wf H))).
+Qed.
+
+(****)
+
+(* A.3 Lemma [Transitivity and Narrowing] *)
+
+(* The statements of the properties of transitivity and narrowing
+   (we give the *statement* here and the *proof* below) *)
+
+Definition transitivity_prop (Q : typ) :=
+  forall (e : env) (S T : typ), sub e S Q -> sub e Q T -> sub e S T.
+
+Definition narrowing_prop (Q : typ) :=
+  forall (e e' : env) (X : nat) (S T : typ),
+  narrow X e e' -> get_bound e X = Some Q ->
+  sub e S T -> sub e' S T.
+
+(* The proof follows closely the paper proof.  However, we cannot
+   perform a proof on the distinguished type [Q] as the induction in
+   the paper proof is on [Q] *up to alpha conversion* (shifting).
+   Instead, we perform a proof by induction on the size of types. *)
+
+Fixpoint size (T : typ) : nat :=
+  match T with
+  | tvar _      => 0
+  | top         => 0
+  | arrow T1 T2 => 1 + size T1 + size T2
+  | all T1 T2   => 1 + size T1 + size T2
+  end.
+
+Lemma shift_preserves_size :
+ forall (T : typ) (X : nat), size (tshift X T) = size T.
+induction T; trivial;
+simpl; intros n; rewrite IHT1; rewrite IHT2; trivial.
+Qed.
+
+(* Now we give the crucial step in the proof of transitivity, showing
+   that transitivity holds if we assume that both transitivity and
+   narrowing hold for smaller "cut types" q' *)
+
+Lemma transitivity_case :
+  forall Q : typ,
+  (forall Q' : typ,
+   size Q' < size Q -> transitivity_prop Q' /\ narrowing_prop Q') ->
+  transitivity_prop Q.
+intros Q H e S T H1 H2; induction H1;
+  [ inversion_clear H2; apply SA_Top; trivial
+  | trivial
+  | exact (SA_Trans_TVar H0 (IHsub H H2))
+  | inversion_clear H2;
+      [ apply SA_Top; trivial;
+        simpl; split;
+          [ apply (proj2 (proj2 (sub_wf H1_)))
+          | apply (proj1 (proj2 (sub_wf H1_0))) ]
+      | apply SA_Arrow;
+          [ assert (H5 : size T1 < size (arrow T1 T2)); try (simpl; omega);
+            generalize (H _ H5); intros (H6, _); exact (H6 _ _ _ H0 H1_)
+          | assert (H5 : size T2 < size (arrow T1 T2)); try (simpl; omega);
+            generalize (H _ H5); intros (H6, _);
+            exact (H6 _ _ _ H1_0 H1) ] ]
+  | inversion_clear H2;
+      [ apply SA_Top; trivial;
+        simpl; split;
+          [ apply (proj2 (proj2 (sub_wf H1_)))
+          | apply wf_typ_ebound with (U := T1);
+            apply (proj1 (proj2 (sub_wf H1_0))) ]
+      | assert (H5 : size T1 < size (all T1 T2)); try (simpl; omega);
+        apply SA_All;
+          [ generalize (H _ H5); intros (H6, _); exact (H6 _ _ _ H0 H1_)
+          | assert (H5' : size (tshift 0 T1) < size (all T1 T2));
+              [ rewrite shift_preserves_size; trivial
+              | generalize (H _ H5'); intros (_, H6);
+                assert (H7 := narrow_0 H0);
+                assert
+                  (H7' : get_bound (ebound e T1) 0 = Some (tshift 0 T1));
+                  [ trivial
+                  | assert (H8 := H6 _ _ _ _ _ H7 H7' H1_0);
+                    assert (H9 : size T2 < size (all T1 T2));
+                    try (simpl; omega);
+                    assert (G1 := proj1 (H _ H9));
+                    exact (G1 (ebound e T0) _ _ H8 H1) ] ] ] ] ].
+Qed.
+
+(* Next we give the crucial step in the proof of narrowing, showing
+   that narrowing for q holds if we assume transitivity for types of
+   the same size as q.  (Not "for q itself" because there is some
+   shifting involved.) *)
+
+Lemma narrowing_case :
+  forall Q : typ,
+  (forall Q' : typ, size Q' = size Q -> transitivity_prop Q') ->
+  narrowing_prop Q.
+intros Q H2 e e' n T1 T2 H3 H4 H5; generalize e' n H3 H4; clear e' n H3 H4;
+generalize Q H2; clear Q H2; induction H5; intros Q H2 e' n H3 H4;
+  [ apply SA_Top;
+      [ exact (narrow_wf_env H3 H)
+      | exact (narrow_wf_typ H3 H0) ]
+  | apply SA_Refl_TVar;
+      [ exact (narrow_wf_env H3 H)
+      | exact (narrow_wf_typ H3 H0) ]
+  | case (eq_nat_dec X n);
+      [ intro E; rewrite E in H; rewrite E; clear X E;
+        assert (H4' := IHsub _ H2 _ _ H3 H4);
+        rewrite H in H4; injection H4; intro E; rewrite E in H4';
+        apply (H2 _ (refl_equal (size Q))) with (2 := H4');
+        rewrite <- E;
+        generalize (get_bound_narrow_eq H3);
+        intros (T1, (T2, (H6, (H7, H8))));
+        rewrite H in H6; injection H6;
+        intro E1; rewrite <- E1 in H8;
+        apply SA_Trans_TVar with (2 := H8); trivial
+      | intro H6; apply SA_Trans_TVar with (2 := IHsub _ H2 _ _ H3 H4);
+        rewrite <- (get_bound_narrow_ne H3 H6); trivial ]
+ | apply SA_Arrow; eauto
+ | apply SA_All;
+     [ eauto
+     | apply IHsub2 with (Q := tshift 0 Q) (n := (1 + n));
+         [ intros Q' E; apply H2; rewrite E; apply shift_preserves_size
+         | apply narrow_extend_bound with (2 := H3);
+           apply narrow_wf_typ with (1 := H3);
+           exact (proj1 (proj2 (sub_wf H5_)))
+         | simpl; rewrite H4; trivial ] ] ].
+Qed.
+
+(* Now we combine the above lemmas into the full proof of transitivity
+   and narrowing, by induction on the size of q.  (Note that this
+   departs slightly from the paper proof, which was by structural
+   induction on q.) *)
+
+Lemma transitivity_and_narrowing :
+ forall Q : typ, transitivity_prop Q /\ narrowing_prop Q.
+assert
+ (H :
+  forall (n : nat) (Q : typ),
+  size Q < n -> transitivity_prop Q /\ narrowing_prop Q);
+ [ induction n;
+    [ intros Q H; assert False; [ omega | contradiction ]
+    | intros Q H; case (le_lt_or_eq _ _ H);
+       [ intro H'; apply IHn; omega
+       | intro E; injection E; clear E; intro E; rewrite <- E in IHn;
+          assert
+           (H1 : forall Q' : typ, size Q' = size Q -> transitivity_prop Q');
+          [ intros Q' E1; rewrite <- E1 in IHn; apply transitivity_case;
+             trivial
+          | split; [ apply H1; trivial | apply narrowing_case; trivial ] ] ] ]
+ | intro Q; apply (H (S (size Q))); omega ].
+Qed.
+
+Lemma sub_transitivity :
+  forall (e : env) (T U V : typ), sub e T U -> sub e U V -> sub e T V.
+intros e T U; apply (proj1 (transitivity_and_narrowing U)).
+Qed.
+
+Lemma sub_narrowing :
+  forall (e e' : env) (X : nat) (S T : typ),
+  narrow X e e' -> sub e S T -> sub e' S T.
+intros e e' n S T H1 H2;
+generalize (get_bound_narrow_eq H1); intros (Q, (P, (H3, _)));
+exact (proj2 (transitivity_and_narrowing Q) _ _ _ _ _ H1 H3 H2).
+Qed.
+
+
+(*************************************************************************)
+(*                              Type safety                              *)
+(*************************************************************************)
+
+
+(*** Substitution of a type variable in an environment ****)
+
+(*
+   This corresponds to the environment operation
+      E, X <: T, E'  |-->  E, [X|->T']E',
+   assuming that E |- T' <: T.
+   (see definition A.9)
+*)
+
+Inductive env_subst : nat -> typ -> env -> env -> Prop :=
+    es_here :
+      forall (e : env) (T T' : typ),
+      sub e T' T -> env_subst 0 T' (ebound e T) e
+  | es_var :
+      forall (X : nat) (T T' : typ) (e e' : env),
+      env_subst X T' e e' ->
+      env_subst X T' (evar e T) (evar e' (tsubst T X T'))
+  | es_bound :
+      forall (X : nat) (T T' : typ) (e e' : env),
+      env_subst X T' e e' ->
+      env_subst (1 + X) (tshift 0 T') (ebound e T) (ebound e' (tsubst T X T')).
+
+Lemma env_subst_get_var :
+  forall (x X' : nat) (e e' : env) (T : typ),
+  (env_subst  X' T e e') ->
+  get_var e' x = opt_map (fun T' => tsubst T' X' T) (get_var e x).
+intros n n' e e' T H; generalize n; clear n; induction H;
+  [ intro n; simpl; induction (get_var e n); simpl; trivial;
+    apply f_equal with (f := @Some typ); apply tsubst_tshift_prop
+  | intro n'; induction n'; simpl; trivial
+  | simpl; intro n'; rewrite IHenv_subst;
+    induction (get_var e n'); simpl; trivial;
+    apply f_equal with (f := @Some typ);
+    apply (tshift_tsubst_prop_1 0 X) ].
+Qed.
+
+Lemma env_subst_get_bound_lt :
+  forall (X X' : nat) (e e' : env) (T : typ),
+  (env_subst X' T e e') -> X < X' ->
+  get_bound e' X = opt_map (fun T' => tsubst T' X' T) (get_bound e X).
+intros n n' e e' T H; generalize n; clear n;
+induction H; simpl; trivial; intros n' H1;
+  [ inversion H1
+  | induction n';
+      [ simpl; apply f_equal with (f := @Some typ);
+        apply (tshift_tsubst_prop_1 0 X)
+      | clear IHn'; rewrite IHenv_subst;
+          [ case (get_bound e n'); simpl; trivial; intro T'';
+            apply f_equal with (f := @Some typ);
+            apply (tshift_tsubst_prop_1 0 X)
+          | omega ] ] ].
+Qed.
+
+Lemma env_subst_get_bound_ge :
+  forall (X X' : nat) (e e' : env) (T : typ),
+  env_subst X' T e e' -> X' < X ->
+  get_bound e' (X - 1) = opt_map (fun T' => tsubst T' X' T) (get_bound e X).
+intros n n' e e' T H; generalize n; clear n;
+induction H; simpl; trivial; intros n' H1;
+  [ induction n';
+      [ inversion H1
+      | simpl; rewrite <- minus_n_O; case (get_bound e n'); simpl; trivial;
+        intro T''; apply f_equal with (f := @Some typ);
+        apply tsubst_tshift_prop ]
+  | induction n';
+      [ inversion H1
+      | clear IHn'; replace ((S n') - 1) with (S (n' - 1)); try omega;
+        rewrite IHenv_subst; try omega;
+        case (get_bound e n'); simpl; trivial; intro T'';
+        apply f_equal with (f := @Some typ);
+        apply (tshift_tsubst_prop_1 0 X) ] ].
+Qed.
+
+Lemma env_subst_wf_typ_0 :
+  forall (e e' : env) (T : typ) (X : nat),
+  env_subst X T e e' -> wf_env e' -> wf_typ e' T.
+intros e e' T X H; induction H; simpl;
+  [ intros _; exact (proj1 (proj2 (sub_wf H)))
+  | intros (H1, H2); apply wf_typ_weakening_var; auto
+  | intros (H1, H2); apply wf_typ_weakening_bound; auto ].
+Qed.
+
+Lemma env_subst_wf_typ :
+  forall (e e' : env) (S T : typ) (X : nat),
+  env_subst X T e e' -> wf_typ e S -> wf_env e' -> wf_typ e' (tsubst S X T).
+intros e e' S; generalize e e'; clear e e'; induction S;
+  [ intros e e' T n' H1 H2 H3; simpl; simpl in H2; case (lt_eq_lt_dec n n');
+      [ intro s; case s; clear s; intro H5;
+          [ simpl; rewrite env_subst_get_bound_lt with (1 := H1) (2 := H5);
+            induction (get_bound e n); trivial; discriminate
+          | exact (env_subst_wf_typ_0 H1 H3) ]
+      | intro H5; simpl;
+        rewrite env_subst_get_bound_ge with (1 := H1) (2 := H5);
+        induction (get_bound e n); trivial; discriminate ]
+  | trivial
+  | simpl; intros e e' T n H0 (H1, H2) H3; eauto
+  | simpl; intros e e' T n H0 (H1, H2) H3; split; eauto;
+    apply IHS2 with (e := (ebound e S1)); trivial;
+      [ exact (es_bound S1 H0)
+      | simpl; split; trivial; apply IHS1 with (1 := H0); trivial ] ].
+Qed.
+
+Lemma env_subst_wf_env :
+  forall (e e' : env) (T : typ) (X : nat),
+  env_subst X T e e' -> wf_env e -> wf_env e'.
+intros e e' T X H; induction H; simpl; try tauto;
+intros (H1, H2); split; auto;
+apply env_subst_wf_typ with (1 := H); auto.
+Qed.
+
+(****)
+
+(*** Typing relation well-formedness ***)
+
+Lemma typing_wf :
+  forall (e : env) (t : term) (U : typ),
+  typing e t U -> wf_env e /\ wf_term e t /\ wf_typ e U.
+intros e t U H; induction H;
+  [ repeat split; simpl; trivial;
+      [ simpl; rewrite H0; discriminate
+      | exact (get_var_wf H H0) ]
+  | simpl in IHtyping; simpl; repeat split; try tauto;
+    apply wf_typ_strengthening_var with (T := T1); tauto
+  | simpl; simpl in IHtyping1; tauto
+  | simpl; simpl in IHtyping; tauto
+  | simpl; simpl in IHtyping; assert (H1 := proj1 (proj2 (sub_wf H0)));
+    repeat split; try tauto;
+    apply env_subst_wf_typ with (1 := es_here H0); tauto
+  | repeat split; try tauto; exact (proj2 (proj2 (sub_wf H0))) ].
+Qed.
+
+(****)
+
+(*** A.4 Lemma [Permutation for Typing] ***)
+
+(* We don't need any permutation lemma. *)
+
+(****)
+
+(*** A.5 Lemma [Weakening for typing] (typing part) ***)
+
+Lemma typing_weakening_bound_ind :
+  forall (e e' : env) (X : nat) (t : term) (U : typ),
+  insert_bound X e e' ->
+  typing e t U -> typing e' (shift_typ X t) (tshift X U).
+intros e e' n t U H1 H2; generalize n e' H1; clear n e' H1;
+induction H2; intros n1 e' H1; simpl;
+  [ apply T_Var;
+      [ exact (insert_bound_wf_env H1 H)
+      | rewrite get_var_insert_bound with (1 := H1); rewrite H0; trivial ]
+  | apply T_Abs; apply IHtyping; apply ib_var; trivial
+  | assert (H2 := (IHtyping1 _ _ H1)); assert (H3 := (IHtyping2 _ _ H1));
+    exact (T_App H2 H3)
+  | apply T_Tabs; apply IHtyping; exact (ib_bound T1 H1)
+  | rewrite (tshift_tsubst_prop_2 0 n1);
+    apply (T_Tapp (IHtyping _ _ H1) (sub_weakening_bound_ind H1 H))
+  | exact (T_Sub (IHtyping _ _ H1) (sub_weakening_bound_ind H1 H)) ].
+Qed.
+
+Lemma typing_weakening_bound :
+  forall (e : env) (t : term) (U V : typ),
+  wf_typ e V -> typing e t U ->
+  typing (ebound e V) (shift_typ 0 t) (tshift 0 U).
+intros e t U V H1 H2; apply typing_weakening_bound_ind with (2 := H2);
+apply ib_here; trivial.
+Qed.
+
+Lemma typing_weakening_var_ind :
+  forall (e : env) (x : nat) (t : term) (U : typ),
+  wf_env e -> typing (remove_var e x) t U -> typing e (shift x t) U.
+intros e n t U H1 H2; cut (exists e', e' = remove_var e n);
+  [ intros (e', E); rewrite <- E in H2; generalize n e E H1; clear n e E H1;
+    induction H2; intros n' e' E H1; simpl;
+      [ apply T_Var; trivial; rewrite E in H0;
+        case (le_gt_dec n' x); intro H2;
+          [ rewrite get_var_remove_var_ge in H0; trivial; omega
+          | rewrite get_var_remove_var_lt in H0; trivial; omega ]
+      | apply T_Abs; apply IHtyping;
+          [ rewrite E; trivial
+          | simpl; split; trivial;
+            assert (H3 := proj1 (proj1 (typing_wf H2))); rewrite E in H3;
+            exact (wf_typ_insert_var H3) ]
+      | exact (T_App (IHtyping1 _ _ E H1) (IHtyping2 _ _ E H1))
+      | apply T_Tabs; apply IHtyping;
+          [ rewrite E; trivial
+          | simpl; split; trivial;
+            assert (H3 := proj1 (proj1 (typing_wf H2))); rewrite E in H3;
+            exact (wf_typ_insert_var H3) ]
+      | apply (T_Tapp (T2 := T2) (IHtyping _ _ E H1));
+        rewrite E in H; exact (sub_weakening_var_ind H1 H)
+      | apply (T_Sub (T2 := T2) (IHtyping _ _ E H1));
+        rewrite E in H; exact (sub_weakening_var_ind H1 H) ]
+  | exists (remove_var e n); trivial ].
+Qed.
+
+Lemma typing_weakening_var :
+  forall (e : env) (t : term) (U V : typ),
+  wf_typ e V -> typing e t U -> typing (evar e V) (shift 0 t) U.
+intros e t U V H1 H2; apply (@typing_weakening_var_ind (evar e V));
+simpl; trivial; split; trivial; exact (proj1 (typing_wf H2)).
+Qed.
+
+(****)
+
+(*** A.6 Lemma [Strengthening] ***)
+
+Lemma sub_strengthening_var :
+  forall (e : env) (x : nat) (U V : typ),
+  sub e U V -> sub (remove_var e x) U V.
+intros e x U V H1; generalize H1; apply sub_extensionality;
+  [ intro X; apply get_bound_remove_var
+  | apply wf_env_remove_var; exact (proj1 (sub_wf H1)) ].
+Qed.
+
+(****)
+
+(*** A.7 Lemma [Narrowing for the Typing Relation] ***)
+
+Lemma typing_narrowing_ind :
+  forall (e e' : env) (X : nat) (t : term) (U : typ),
+  narrow X e e' -> typing e t U -> typing e' t U.
+intros e e' n t U H1 H2; generalize e' n H1; clear e' n H1;
+induction H2; intros e' n1 H1;
+  [ apply T_Var;
+      [ exact (narrow_wf_env H1 H)
+      | rewrite <- get_var_narrow with (1 := H1); trivial ]
+  | apply T_Abs; apply IHtyping with (n := n1);
+    apply narrow_extend_var; trivial;
+    exact (narrow_wf_typ H1 (proj1 (proj1 (typing_wf H2))))
+  | eapply T_App; eauto
+  | apply T_Tabs; apply IHtyping with (n := S n1);
+    apply narrow_extend_bound with (X := n1); trivial;
+    exact (narrow_wf_typ H1 (proj1 (proj1 (typing_wf H2))))
+  | eapply T_Tapp; eauto; exact (sub_narrowing H1 H)
+  | apply T_Sub with (1 := IHtyping _ _ H1); exact (sub_narrowing H1 H) ].
+Qed.
+
+Lemma typing_narrowing :
+ forall (e : env) (t : term) (U V1 V2 : typ),
+ typing (ebound e V1) t U -> sub e V2 V1 -> typing (ebound e V2) t U.
+intros e t U V1 V2 H1 H2; exact (typing_narrowing_ind (narrow_0 H2) H1).
+Qed.
+
+(****)
+
+(*** A.8 Lemma [Subtyping preserves typing] ***)
+
+(* Compared to the lemma in the paper proof, this lemma is slightly
+   stronger: [u] is typed in a larger environment.  This makes it
+   possible to use our one-step weakning lemmas rather that the
+   stronger lemmas of the paper proof. *)
+
+Lemma subst_preserves_typing :
+  forall (e : env) (x : nat) (t u : term) (V W : typ),
+  typing e t V ->
+  typing (remove_var e x) u W -> get_var e x = Some W ->
+  typing (remove_var e x) (subst t x u) V.
+intros e n t u V W H; generalize n u W; clear n u W;
+induction H; intros n' u W H1 E1;
+  [ simpl; case (lt_eq_lt_dec x n');
+      [ intro s; case s; clear s; intro H2;
+          [ apply T_Var;
+              [ apply wf_env_remove_var; trivial
+              | rewrite get_var_remove_var_lt with (1 := H2); trivial ]
+          | rewrite H2 in H0; rewrite H0 in E1; injection E1;
+            intro E3; rewrite E3; trivial ]
+      | intro H2; apply T_Var;
+          [ apply wf_env_remove_var; trivial
+          | induction x;
+              [ inversion H2
+              | simpl; rewrite <- minus_n_O;
+                rewrite get_var_remove_var_ge; trivial; omega ] ] ]
+  | simpl; apply T_Abs; apply (IHtyping (S n') (shift 0 u) W); trivial;
+    assert (H2 := wf_typ_remove_var n' (proj1 (proj1 (typing_wf H))));
+    exact (typing_weakening_var H2 H1)
+  | exact (T_App (IHtyping1 _ u W H1 E1) (IHtyping2 _ u W H1 E1))
+  | simpl; apply T_Tabs; apply (IHtyping n' (shift_typ 0 u) (tshift 0 W));
+      [ assert (H2 := wf_typ_remove_var n' (proj1 (proj1 (typing_wf H))));
+        exact (typing_weakening_bound H2 H1)
+      | simpl; rewrite E1; trivial ]
+  | simpl; apply T_Tapp with (1 := (IHtyping _ u W H1 E1));
+    exact (sub_strengthening_var n' H0)
+  | simpl; apply T_Sub with (1 := (IHtyping _ u W H1 E1));
+    exact (sub_strengthening_var n' H0) ].
+Qed.
+
+(****)
+
+(*** A.10 Lemma [Type substitution preserves subtyping] ***)
+
+Lemma env_subst_sub :
+  forall (e e' : env) (T T' : typ) (X : nat),
+  env_subst X T' e e' -> (get_bound e X) = (Some T) -> wf_env e' ->
+  (sub e' T' (tsubst T X T')).
+intros e e' T T' X H; generalize T; clear T; induction H; simpl;
+  [ intros T'' E H1; injection E; clear E; intro E; rewrite <- E;
+    rewrite <- tsubst_tshift_prop; trivial
+  | intros T'' E (H1, H2);
+    exact (sub_weakening_var H1 (IHenv_subst _ E H2))
+  | intros T'' E (H1, H2); induction (get_bound e X); try discriminate;
+    injection E; clear E; intro E; rewrite <- E;
+    rewrite <- (tshift_tsubst_prop_1 0 X);
+    apply sub_weakening_bound with (1 := H1); auto ].
+Qed.
+
+Lemma tsubst_preserves_subtyping :
+  forall (e e' : env) (X : nat) (T U V : typ),
+  env_subst X T e e' -> sub e U V -> sub e' (tsubst U X T) (tsubst V X T).
+intros e e' n T U V H1 H2; generalize n e' T H1; clear n e' T H1; induction H2;
+  [ intros n e' T H1; apply SA_Top;
+      [ exact (env_subst_wf_env H1 H)
+      | exact (env_subst_wf_typ H1 H0 (env_subst_wf_env H1 H)) ]
+  | intros n e' T H1; apply sub_reflexivity;
+      [ exact (env_subst_wf_env H1 H)
+      | exact (env_subst_wf_typ H1 H0 (env_subst_wf_env H1 H)) ]
+  | intros n e' T' H1; simpl; case (lt_eq_lt_dec X n);
+      [ intros s; case s; clear s;
+          [ intro H5; apply SA_Trans_TVar with (U := tsubst U n T');
+              [ rewrite env_subst_get_bound_lt with (1 := H1) (2 := H5);
+                rewrite H; trivial
+              | apply IHsub; trivial ]
+          | intro E; apply sub_transitivity with (2 := IHsub _ _ _ H1);
+            rewrite E in H; apply (env_subst_sub H1 H);
+            exact (env_subst_wf_env H1 (proj1 (sub_wf H2))) ]
+      | intro H5; apply SA_Trans_TVar with (U := tsubst U n T');
+          [ rewrite env_subst_get_bound_ge with (1 := H1); try omega;
+            induction X;
+              [ assert False; [ omega | contradiction ]
+              | simpl; rewrite H; trivial ]
+          | apply IHsub; trivial ] ]
+  | intros n e' T H1; simpl; apply SA_Arrow; auto
+  | intros n e' T H1; simpl; apply SA_All; auto;
+    exact (IHsub2 _ _ _ (es_bound T1 H1)) ].
+Qed.
+
+(****)
+
+(* A.11 Lemma [Type substitution preserves typing] *)
+
+Lemma subst_typ_preserves_typing_ind :
+  forall (e e' : env) (t : term) (U P : typ) (X : nat),
+  env_subst X P e e' ->
+  typing e t U -> typing e' (subst_typ t X P) (tsubst U X P).
+intros e e' t U P n H1 H2; generalize n e' P H1; clear n e' P H1;
+induction H2;
+  [ intros n' e' P H1; simpl; apply T_Var;
+      [ exact (env_subst_wf_env H1 H)
+      | rewrite env_subst_get_var with (1 := H1); rewrite H0; trivial ]
+  | intros n e' P H1; simpl; apply T_Abs; exact (IHtyping _ _ _ (es_var _ H1))
+  | intros n e' P H1; exact (T_App (IHtyping1 _ _ _ H1) (IHtyping2 _ _ _ H1))
+  | intros n e' P H1; exact (T_Tabs (IHtyping _ _ _ (es_bound _ H1)))
+  | intros n e' P H1; simpl;
+    assert (H4 := T_Tapp (T2 := (tsubst T2 n P)) (IHtyping _ _ _ H1));
+    fold tsubst in H4; rewrite (tsubst_tsubst_prop 0 n);
+    apply H4; exact (tsubst_preserves_subtyping H1 H)
+  | intros n e' P H1; apply T_Sub with (1 := IHtyping _ _ _ H1);
+    exact (tsubst_preserves_subtyping H1 H) ].
+Qed.
+
+Lemma subst_typ_preserves_typing :
+  forall (e : env) (t : term) (U P Q : typ),
+  typing (ebound e Q) t U -> sub e P Q ->
+  typing e (subst_typ t 0 P) (tsubst U 0 P).
+intros e t U P Q H1 H2; exact (subst_typ_preserves_typing_ind (es_here H2) H1).
+Qed.
+
+(****)
+
+(*** A.12 Lemma [Inversion of subtyping] ***)
+
+(* We use Coq inversion tactics instead. *)
+
+(****)
+
+(*** A.13 Lemma ***)
+
+Lemma t_abs_inversion :
+  forall (e : env) (t : term) (T0 T1 T2 T3 : typ),
+  typing e (abs T1 t) T0 ->
+  sub e T0 (arrow T2 T3) ->
+  sub e T2 T1 /\
+  (exists T4, sub e T4 T3 /\ typing (evar e T1) t T4).
+intros e t T0 T1 T2 T3 H; cut (exists t' : _, t' = abs T1 t);
+  [ intros (t', E1); rewrite <- E1 in H; generalize t T1 T2 T3 E1;
+    clear t T1 T2 T3 E1;
+    induction H; intros; try discriminate;
+      [ injection E1; intros E2 E3; rewrite <- E2; rewrite <- E3;
+        inversion_clear H0; split; [ trivial | exists T2; split; trivial ]
+      | apply IHtyping with (1 := E1) (2 := sub_transitivity H0 H1) ]
+  | exists (abs T1 t); trivial ].
+Qed.
+
+Lemma t_tabs_inversion :
+  forall (e : env) (t : term) (T0 T1 T2 T3 : typ),
+  typing e (tabs T1 t) T0 ->
+  sub e T0 (all T2 T3) ->
+  sub e T2 T1 /\
+  (exists T4, sub (ebound e T2) T4 T3 /\ typing (ebound e T2) t T4).
+intros e t T0 T1 T2 T3 H; cut (exists t' : _, t' = tabs T1 t);
+  [ intros (t', E1); rewrite <- E1 in H; generalize t T1 T2 T3 E1;
+    clear t T1 T2 T3 E1;
+    induction H; intros; try discriminate;
+      [ injection E1; intros E2 E3; rewrite <- E2; rewrite <- E3;
+        inversion_clear H0; split; trivial;
+        exists T2; split; trivial; exact (typing_narrowing H H1)
+      | apply IHtyping with (1 := E1) (2 := sub_transitivity H0 H1) ]
+  | exists (tabs T1 t); trivial ].
+Qed.
+
+(****)
+
+(*** A.14 Lemma [Canonical Forms] ***)
+
+Lemma fun_value :
+  forall (t : term) (T1 T2 : typ),
+  value t -> typing empty t (arrow T1 T2) ->
+  exists t' , exists T1' , t = abs T1' t'.
+intros t T1 T2 H1 H; cut (exists e, e = empty);
+  [ intros (e, E1); rewrite <- E1 in H; cut (exists T0, T0 = arrow T1 T2);
+      [ intros (T0, E2); rewrite <- E2 in H; generalize T1 T2 E2;
+        clear T1 T2 E2; induction H; try contradiction;
+          [ intros T3 T4 E; exists t; exists T1; trivial
+          | intros; discriminate
+          | intros T3 T4 E2; rewrite E2 in H0; inversion H0;
+              [ rewrite E1 in H2; induction X; discriminate
+              | exact (IHtyping H1 E1 _ _ (sym_eq H5)) ] ]
+      | exists (arrow T1 T2); trivial ]
+  | exists empty; trivial ].
+Qed.
+
+Lemma typefun_value :
+  forall (t : term) (T1 T2 : typ),
+  value t -> typing empty t (all T1 T2) ->
+  exists t', exists T1', t = tabs T1' t'.
+intros t T1 T2 H1 H; cut (exists e, e = empty);
+  [ intros (e, E1); rewrite <- E1 in H; cut (exists T0, T0 = all T1 T2);
+      [ intros (T0, E2); rewrite <- E2 in H; generalize T1 T2 E2;
+        clear T1 T2 E2; induction H; try contradiction;
+          [ intros; discriminate
+          | intros T3 T4 E; exists t; exists T1; trivial
+          | intros T3 T4 E2; rewrite E2 in H0; inversion H0;
+              [ rewrite E1 in H2; induction X; discriminate
+              | exact (IHtyping H1 E1 _ _ (sym_eq H5)) ] ]
+      | exists (all T1 T2); trivial ]
+  | exists empty; trivial ].
+Qed.
+
+(****)
+
+(*** A.15 Lemma ***)
+
+Lemma local_progress :
+  forall (t : term) (U : typ),
+  typing empty t U -> value t \/
+  exists c, exists t0, exists t0', red t0 t0' /\ t = ctx_app c t0.
+intros t U H; cut (exists e, e = empty);
+  [ intros (e, E); rewrite <- E in H;
+    induction H;
+      [ rewrite E in H0; induction x; discriminate
+      | simpl; auto
+      | right; case (IHtyping1 E); clear IHtyping1;
+          [ intro H2; case (IHtyping2 E); clear IHtyping2;
+              [ intro H3; rewrite E in H; generalize (fun_value H2 H);
+                intros (t', (T1', E1)); rewrite E1; exists c_hole;
+                exists (app (abs T1' t') t2); exists (subst t' 0 t2);
+                split; trivial; apply E_AppAbs; trivial
+              | intros (c, (t0, (t0', (H3, E1)))); exists (c_apparg H2 c);
+                exists t0; exists t0'; rewrite E1; auto ]
+          | intros (c, (t0, (t0', (H3, E1)))); exists (c_appfun c t2);
+            exists t0; exists t0'; rewrite E1; auto ]
+      | simpl; auto
+      | right; case (IHtyping E); clear IHtyping;
+          [ intro H1; rewrite E in H; generalize (typefun_value H1 H);
+            intros (t', (T1', E1)); rewrite E1; exists c_hole;
+            exists (tapp (tabs T1' t') T2); exists (subst_typ t' 0 T2);
+            split; trivial; apply E_TappTabs
+          | intros (c, (t0, (t0', (H3, E1)))); exists (c_typefun c T2);
+            exists t0; exists t0'; rewrite E1; auto ]
+      | auto ]
+  | exists empty; trivial ].
+Qed.
+
+(****)
+
+(*** A.16 Theorem [Progress] ***)
+
+Theorem progress :
+  forall (t : term) (U : typ),
+  typing empty t U -> value t \/ exists t', red t t'.
+intros t U H; generalize (local_progress H);
+intros [H1 | (c, (t0, (t0', (H1, H2))))]; auto;
+right; exists (ctx_app c t0'); rewrite H2; apply E_Ctx; trivial.
+Qed.
+
+(****)
+
+(*** A.18 Lemma ***)
+
+(*
+   We only prove the first part of the lemma, as the second part is
+   not needed.
+   We don't follow the paper proof sketch (induction on the structure
+   of evaluation contexts, then case on the last rule used in the
+   typing derivation) as this does not go through...  Instead, our
+   proof is by induction on the typing derivation and case on the
+   evaluation context.
+*)
+
+Lemma context_replacement :
+   forall (e : env) (c : ctx) (t t' : term) (T : typ),
+   (forall (T' : typ), (typing e t T') -> (typing e t' T')) ->
+   typing e (ctx_app c t) T -> typing e (ctx_app c t') T.
+intros e c t t' T H1 H2; cut (exists t'', t'' = ctx_app c t);
+  [ intros (t'', E); rewrite <- E in H2;
+    generalize c E; clear c E; induction H2;
+      [ induction c; try (intros; discriminate); simpl;
+        intros E; apply H1; rewrite <- E; apply T_Var; trivial
+      | induction c; try (intros; discriminate); simpl;
+        intros E; apply H1; rewrite <- E; apply T_Abs; trivial
+      | induction c; try (intros; discriminate); simpl;
+          [ intros E; apply H1; rewrite <- E; exact (T_App H2_ H2_0)
+          | intro E; injection E; clear E; intros E1 E2;
+            rewrite <- E1; apply T_App with (2 := H2_0);
+            apply IHtyping1; trivial
+          | intro E; injection E; clear E; intros E1 E2;
+            rewrite <- E2; apply T_App with (1 := H2_);
+            apply IHtyping2; trivial ]
+      | induction c; try (intros; discriminate); simpl;
+        intros E; apply H1; rewrite <- E; exact (T_Tabs H2)
+      | induction c; try (intros; discriminate); simpl;
+          [ intros E; apply H1; rewrite <- E; exact (T_Tapp H2 H)
+          | intro E; injection E; clear E; intros E1 E2;
+            rewrite <- E1; apply T_Tapp with (2 := H);
+            apply IHtyping; trivial ]
+      | intros c E; apply T_Sub with (2 := H); apply IHtyping; trivial ]
+  | exists (ctx_app c t); trivial ].
+Qed.
+
+(****)
+
+(*** A.18 Lemma ***)
+
+Lemma local_preservation_app :
+  forall (e : env) (t12 t2 : term) (T11 U : typ),
+  typing e (app (abs T11 t12) t2) U -> typing e (subst t12 0 t2) U.
+intros e t12 t2 T11 U H; cut (exists t, t = app (abs T11 t12) t2);
+  [ intros (t, E); rewrite <- E in H; induction H; try discriminate;
+      [ injection E; clear E; intros E1 E2; rewrite E2 in H;
+        assert (H6 := proj1 (typing_wf H));
+        assert (H7 := proj2 (proj2 (typing_wf H)));
+        generalize (t_abs_inversion H (sub_reflexivity H6 H7));
+        intros (H2, (T4, (H4, H5))); apply T_Sub with (2 := H4);
+        apply (subst_preserves_typing (x := 0) (u := t2) (W := T11) H5);
+        trivial; simpl; rewrite <- E1; exact (T_Sub H0 H2)
+      | apply T_Sub with (2 := H0); auto ]
+  | exists (app (abs T11 t12) t2); trivial ].
+Qed.
+
+Lemma local_preservation_tapp :
+  forall (e : env) (t12 : term) (T11 T2 U : typ),
+  typing e (tapp (tabs T11 t12) T2) U -> typing e (subst_typ t12 0 T2) U.
+intros e t12 T11 T2 U H; cut (exists t, t = tapp (tabs T11 t12) T2);
+  [ intros (t, E); rewrite <- E in H; induction H; try discriminate;
+      [ injection E; clear E; intros E1 E2; rewrite E2 in H;
+        assert (H7 := proj1 (typing_wf H));
+        assert (H8 := proj2 (proj2 (typing_wf H)));
+        generalize (t_tabs_inversion H (sub_reflexivity H7 H8));
+        intros (H2, (T3, (H4, H5))); assert (H6 := T_Sub H5 H4);
+        rewrite <- E1; exact (subst_typ_preserves_typing H6 H0)
+      | apply T_Sub with (2 := H0); auto ]
+  | exists (tapp (tabs T11 t12) T2); trivial ].
+Qed.
+
+(****)
+
+(*** A.20 Theorem [Preservation] ***)
+
+Theorem preservation :
+  forall (e : env) (t t' : term) (U : typ),
+  typing e t U -> red t t' -> typing e t' U.
+intros e t t' U H1 H2; generalize U H1; clear U H1; induction H2; intros U H1;
+  [ exact (local_preservation_app H1)
+  | exact (local_preservation_tapp H1)
+  | exact (context_replacement IHred H1) ].
+Qed.
+
+
+(*************************************************************************)
+(*                      Alternate reduction relation                     *)
+(*************************************************************************)
+
+
+Inductive red' : term -> term -> Prop :=
+  | appabs :
+      forall (t11 : typ) (t12 t2 : term),
+      value t2 -> red' (app (abs t11 t12) t2) (subst t12 0 t2)
+  | tapptabs :
+      forall (t11 t2 : typ) (t12 : term),
+      red' (tapp (tabs t11 t12) t2) (subst_typ t12 0 t2)
+  | appfun :
+      forall t1 t1' t2 : term, red' t1 t1' -> red' (app t1 t2) (app t1' t2)
+  | apparg :
+      forall t1 t2 t2' : term,
+      value t1 -> red' t2 t2' -> red' (app t1 t2) (app t1 t2')
+  | typefun :
+      forall (t1 t1' : term) (t2 : typ),
+      red' t1 t1' -> red' (tapp t1 t2) (tapp t1' t2).
+
+Theorem progress' :
+  forall (t : term) (U : typ),
+  typing empty t U -> value t \/ exists t', red' t t'.
+intros t U H; cut (exists e, e = empty);
+  [ intros (e, E); rewrite <- E in H;
+    induction H;
+      [ rewrite E in H0; induction x; discriminate
+      | simpl; auto
+      | right; case (IHtyping1 E);
+          [ intro H2; case (IHtyping2 E);
+              [ intro H3; rewrite E in H; generalize (fun_value H2 H);
+                intros (t', (T1', E1)); rewrite E1; exists (subst t' 0 t2);
+                apply appabs; trivial
+              | intros (t2', H3); exists (app t1 t2'); apply apparg; trivial ]
+          | intros (t1', H2); exists (app t1' t2); apply appfun; trivial ]
+      | simpl; auto
+      | right; case (IHtyping E);
+          [ intro H1; rewrite E in H; generalize (typefun_value H1 H);
+            intros (t', (T1', E1)); rewrite E1; exists (subst_typ t' 0 T2);
+            apply tapptabs; trivial
+          | intros (t1', H1); exists (tapp t1' T2); apply typefun; trivial ]
+      | auto ]
+  | exists empty; trivial ].
+Qed.
+
+Theorem preservation' :
+  forall (e : env) (t t' : term) (U : typ),
+  typing e t U -> red' t t' -> typing e t' U.
+intros e t t' U H1; generalize t'; clear t'; induction H1;
+  [ intros t' H1; inversion_clear H1
+  | intros t' H2; inversion_clear H2
+  | intros t' H2; generalize H1_ IHtyping1; clear H1_ IHtyping1;
+    inversion_clear H2;
+      [ intros H1 IHtyping1;
+        assert (H6 := proj1 (typing_wf H1));
+        assert (H7 := proj2 (proj2 (typing_wf H1)));
+        generalize (t_abs_inversion H1 (sub_reflexivity H6 H7));
+        intros (H2, (T4, (H4, H5))); apply T_Sub with (2 := H4);
+        apply (subst_preserves_typing (x := 0) (u := t2) (W := t11) H5);
+        trivial; simpl; exact (T_Sub H1_0 H2)
+      | intros H1 IHtyping1; apply T_App with (1 := IHtyping1 _ H); trivial
+      | intros H2 IHtyping1; apply T_App with (2 := IHtyping2 _ H0); trivial ]
+  | intros t' H2; inversion_clear H2
+  | intros t' H2; generalize H1 IHtyping; clear H1 IHtyping;
+    inversion_clear H2; intros H1 IHtyping;
+      [ assert (H7 := proj1 (typing_wf H1));
+        assert (H8 := proj2 (proj2 (typing_wf H1)));
+        generalize (t_tabs_inversion H1 (sub_reflexivity H7 H8));
+        intros (H2, (T3, (H4, H5))); assert (H6 := T_Sub H5 H4);
+        exact (subst_typ_preserves_typing H6 H)
+      | apply T_Tapp with (1 := IHtyping _ H0); trivial ]
+  | intros t' H2; eapply T_Sub; auto ].
+Qed.
